{
 "cells": [
  {
   "cell_type": "markdown",
   "metadata": {},
   "source": [
    "# Complex Analysis, Priestly Question 1.8\n",
    "\n",
    "Evaluate $\\sum_{k=1}^n e^{ik\\theta}$.  Deduce that:\n",
    "\n",
    "$$-1 + 2\\sum_{k=1}^n \\cos k\\theta = \\frac{\\sin \\left(n + \\frac{1}{2}\\right)n}{\\sin \\frac{1}{2} \\theta} \\text{ for } \\theta \\neq 2m\\pi ( m\\in \\mathbb{Z} )\\;.$$\n",
    "\n",
    "Find a similar expression for $\\sum_{k=1}^n \\sin k\\theta$."
   ]
  },
  {
   "cell_type": "markdown",
   "metadata": {},
   "source": [
    "Solution:\n",
    "\n",
    "When $\\theta \\neq 2m\\pi$, $\\sin \\frac{1}{2}\\theta \\neq 0$ so there is no division by 0.\n",
    "\n",
    "Recall the geometric series formula:\n",
    "$$\\sum_{k=0}^n r^k = \\frac{1-r^{n+1}}{1-r}\\;,$$\n",
    "and let $r = e^{i\\theta}$:\n",
    "$$\\sum_{k=0}^n e^{i\\theta k} = \\frac{1-e^{i(n+1)\\theta}}{1-e^{i\\theta}}\\;,$$\n",
    "\n",
    "Since \n",
    "\n",
    "\\begin{align*}\n",
    "e^{i\\theta} &= \\cos k\\theta + i\\sin \\theta\\\\\n",
    "e^{-i\\theta} &=  \\cos k\\theta -i\\sin \\theta\\;,\\\\\n",
    "\\end{align*}\n",
    "\n",
    "we can substitute these expressions in to the geometric series formula:\n",
    "\\begin{align*}\n",
    "\\sum_{k=0}^n e^{ik\\theta} =\\frac{1-\\cos (n+1) \\theta +i \\sin (n+1)\\theta}{1-\\cos\\theta - i \\sin \\theta} \\\\\n",
    "\\sum_{k=0}^n e^{-ik\\theta} =\\frac{1-\\cos (n+1) \\theta - i \\sin (n+1)\\theta}{1-\\cos\\theta + i \\sin \\theta} \\\\\n",
    "\\end{align*}\n",
    "\n",
    "In addition, we have:\n",
    "\\begin{align*}\n",
    "\\sum_{k=0}^n e^{ik\\theta} &= \\sum_{k=0}^n \\left( \\cos k\\theta + i\\sin k\\theta \\right)\\\\\n",
    " \\sum_{k=0}^n e^{-ik\\theta} &=  \\sum_{k=0}^n \\left( \\cos k\\theta -i\\sin k\\theta \\right)\\;.\\\\\n",
    "\\end{align*}\n",
    "\n",
    "Therefore, we can get a summation for cosine by adding the above summations:\n",
    "\n",
    "$$ 2\\sum_{k=0}^n \\cos k\\theta = \\sum_{k=0}^n e^{ik\\theta} +  \\sum_{k=0}^n e^{-ik\\theta} $$\n",
    "\n",
    "Before adding the two summations, we first simplify them further.  The summation $\\sum_{k=0}^n e^{ik\\theta}$ simplifies as follows:\n",
    "\n",
    "\\begin{align*}\n",
    "\\sum_{k=0}^n e^{ik\\theta} &=\\frac{1-\\cos (n+1) \\theta - i \\sin (n+1)\\theta}{1-\\cos\\theta - i \\sin \\theta} \\\\\n",
    "&=\\frac{1-\\cos (n+1) \\theta - i \\sin (n+1)\\theta}{1-\\cos\\theta - i \\sin \\theta} \\times \\frac{1-\\cos \\theta + i \\sin \\theta}{1-\\cos \\theta + i \\sin \\theta} \\\\\n",
    "&= \\frac{(1-\\cos(n+1)\\theta)(1-\\cos \\theta) + \\sin(n+1)\\theta\\sin\\theta}{(1-\\cos \\theta)^2 + \\sin^2\\theta} + i\\frac{\\sin\\theta(1-\\cos(n+1)\\theta) -\\sin(n+1)\\theta(1-\\cos\\theta)}{(1-\\cos \\theta)^2 + \\sin^2\\theta}\n",
    "\\end{align*}\n",
    "\n",
    "The summation $\\sum_{k=0}^n e^{-ik\\theta}$ simplify as follows:\n",
    "\n",
    "\\begin{align*}\n",
    "\\sum_{k=0}^n e^{-ik\\theta} &=\\frac{1-\\cos (n+1) \\theta - i \\sin (n+1)\\theta}{1-\\cos\\theta + i \\sin \\theta}\\times \\frac{1-\\cos \\theta- i \\sin \\theta}{1-\\cos \\theta - i \\sin \\theta} \\\\\n",
    "&=\\frac{(1-\\cos(n+1)\\theta)(1-\\cos\\theta)+\\sin(n+1)\\theta \\sin\\theta}{(1-\\cos \\theta)^2 + \\sin^2\\theta} - i\\frac{\\sin\\theta(1-\\cos(n+1)\\theta) -\\sin(n+1)\\theta(1-\\cos\\theta)}{(1-\\cos \\theta)^2 + \\sin^2\\theta}\n",
    "\\end{align*}\n",
    "\n",
    "Now we have the expression for $\\sum_{k=0}^n \\cos k\\theta$:\n",
    "\n",
    "$$2\\sum_{k=0}^n \\cos k\\theta = 2\\frac{(1-\\cos(n+1)\\theta)(1-\\cos\\theta)+\\sin(n+1)\\theta \\sin\\theta}{(1-\\cos \\theta)^2  + \\sin^2\\theta}\\;.$$\n",
    "\n",
    "The denominator can be further simplified:\n",
    "\\begin{align*}\n",
    "&(1-\\cos \\theta)^2  + \\sin^2\\theta \\\\\n",
    "&=1-2\\cos\\theta + \\cos^2 \\theta + \\sin^2\\theta \\\\\n",
    "&= 2(1-\\cos \\theta)\\;.\n",
    "\\end{align*}\n",
    "\n",
    "The following trigonometric identities will help us to further simplify this expression:\n",
    "\n",
    "\\begin{align*}\n",
    "\\sin(u \\pm v) &= \\sin u \\cos v \\pm \\cos u \\sin v \\;, \\\\\n",
    "\\cos(u \\pm v) &= \\cos u \\cos v \\mp \\sin u \\sin v \\;, \\\\\n",
    "\\sin 2u &= 2 \\sin u \\cos u \\;,\\\\\n",
    "\\sin^2 u &= \\frac{1-cos 2u}{2}\\;,\n",
    "\\end{align*}\n",
    "\n",
    "Using all of the above equations, the simplification proceeds as follows:\n",
    "\n",
    "\\begin{align*}\n",
    "2\\sum_{k=0}^n \\cos k\\theta &= 2\\frac{(1-\\cos(n+1)\\theta)(1-\\cos\\theta)+\\sin(n+1)\\theta \\sin\\theta}{(1-\\cos \\theta)^2  + \\sin^2\\theta} \\\\\n",
    "&= \\frac{ (1-\\cos(n+1)\\theta)(1-\\cos\\theta)+\\sin(n+1)\\theta \\sin\\theta)}{2(1-\\cos\\theta)} \\\\\n",
    "&= \\frac{ 1-\\cos\\theta-\\cos(n+1)\\theta + \\cos(n+1)\\theta \\cos\\theta+\\sin(n+1)\\theta \\sin\\theta}{1-\\cos\\theta}\\\\\n",
    "&= \\frac{ 1-\\cos\\theta-\\cos(n+1)\\theta+ \\cos(n+1)\\theta \\cos\\theta+\\sin(n+1)\\theta \\sin\\theta}{1-\\cos\\theta}\\\\\n",
    "&= \\frac{ 1-\\cos\\theta-\\cos(n+1)\\theta+ \\cos n\\theta }{1-\\cos\\theta}\\\\\n",
    "&= 1-\\frac{ \\cos(n+1)\\theta- \\cos n\\theta }{1-\\cos\\theta}\\\\\n",
    "&= 1-\\frac{ \\cos n\\theta \\cos \\theta - \\sin n\\theta\\sin\\theta- \\cos n\\theta }{1-\\cos\\theta}\\\\\n",
    "&= 1+\\frac{ \\cos n\\theta - \\cos n\\theta \\cos \\theta +\\sin n\\theta\\sin\\theta}{1-\\cos\\theta}\\\\\n",
    "&= 1+\\frac{ \\cos n\\theta(1 - \\cos \\theta) + \\sin n\\theta\\sin\\theta}{1-\\cos\\theta}\\\\\n",
    "&= 1+\\frac{ \\cos n\\theta (2\\sin^2\\frac{\\theta}{2}) + \\sin n\\theta(2\\sin\\frac{\\theta}{2}\\cos\\frac{\\theta}{2})}{2\\sin^2\\frac{\\theta}{2}}\\\\\n",
    "&= 1+\\frac{ \\cos n\\theta \\sin\\frac{\\theta}{2} + \\sin n\\theta \\cos\\frac{\\theta}{2}}{\\sin\\frac{\\theta}{2}}\\\\\n",
    "&= 1+\\frac{ \\sin \\left(n+\\frac{1}{2}\\right) \\theta}{\\sin\\frac{\\theta}{2}}\\\\\n",
    "\\end{align*}\n",
    "\n",
    "Moving the 1 to the left hand side concludes the simplification:\n",
    "$$-1 + 2\\sum_{k=0}^n \\cos k\\theta = \\frac{ \\sin \\left(n+\\frac{1}{2}\\right) \\theta}{\\sin\\frac{\\theta}{2}} $$\n"
   ]
  },
  {
   "cell_type": "code",
   "execution_count": null,
   "metadata": {},
   "outputs": [],
   "source": []
  }
 ],
 "metadata": {
  "kernelspec": {
   "display_name": "Python 3",
   "language": "python",
   "name": "python3"
  },
  "language_info": {
   "codemirror_mode": {
    "name": "ipython",
    "version": 3
   },
   "file_extension": ".py",
   "mimetype": "text/x-python",
   "name": "python",
   "nbconvert_exporter": "python",
   "pygments_lexer": "ipython3",
   "version": "3.8.5"
  }
 },
 "nbformat": 4,
 "nbformat_minor": 4
}
